progress including framedness information in method call rule
* showed that precondition is framed, need to still prove auxiliary lemma showing that expression evaluation stays the same if the states differ only on variables that are not free in the expression
* still need to show that postcondition is framed

TotalUtil.thy
@@ -990,4 +990,44 @@ abbreviation no_unfolding_pure_exp
 abbreviation no_unfolding_assertion
   where "no_unfolding_assertion \<equiv> assert_pred (\<lambda>_. True) (\<lambda>_. True) no_unfolding_pure_exp_no_rec"
 
+subsection \<open>Free variables\<close>
+
+fun free_var_pure_exp :: "pure_exp \<Rightarrow> var set"
+  where
+  "free_var_pure_exp (Var x) = {x}"
+| "free_var_pure_exp (ELit lit) = {}"
+| "free_var_pure_exp Result = {}"
+| "free_var_pure_exp (Unop uop e) = free_var_pure_exp e"
+| "free_var_pure_exp (Binop e1 bop e2) = free_var_pure_exp e1 \<union> free_var_pure_exp e2"
+| "free_var_pure_exp (CondExp cond e1 e2) = free_var_pure_exp cond \<union> free_var_pure_exp e1 \<union> free_var_pure_exp e2"
+| "free_var_pure_exp (FieldAcc e f) = free_var_pure_exp e"
+| "free_var_pure_exp (Old lbl e) = free_var_pure_exp e"
+| "free_var_pure_exp (Perm e f) = free_var_pure_exp e"
+| "free_var_pure_exp (PermPred pname es) = \<Union> (set (map free_var_pure_exp es))"
+| "free_var_pure_exp (FunApp f es) = \<Union> (set (map free_var_pure_exp es))"
+| "free_var_pure_exp (Unfolding pname es e) = \<Union> (set (map free_var_pure_exp es)) \<union> free_var_pure_exp e"
+| "free_var_pure_exp (pure_exp.Let e e_body) = undefined" \<comment>\<open>TODO\<close>
+| "free_var_pure_exp (PExists ty e) = undefined" \<comment>\<open>TODO\<close>
+| "free_var_pure_exp (PForall ty e) = undefined" \<comment>\<open>TODO\<close>
+
+fun
+  free_var_atomic_assert :: "pure_exp atomic_assert \<Rightarrow> var set" where  
+  "free_var_atomic_assert (Pure e) = free_var_pure_exp e"
+| "free_var_atomic_assert (Acc e f Wildcard) = free_var_pure_exp e"
+| "free_var_atomic_assert (Acc e1 f (PureExp e2)) = free_var_pure_exp e1 \<union> free_var_pure_exp e2"
+| "free_var_atomic_assert (AccPredicate pname es Wildcard) = \<Union> (set (map free_var_pure_exp es))"
+| "free_var_atomic_assert (AccPredicate pname es (PureExp e2)) = \<Union> (set (map free_var_pure_exp es)) \<union> free_var_pure_exp e2"
+
+fun free_var_assertion :: "assertion \<Rightarrow> var set"  where  
+  "free_var_assertion (Atomic atm) = free_var_atomic_assert atm"
+| "free_var_assertion (Imp e A) = free_var_pure_exp e \<union> free_var_assertion A"
+| "free_var_assertion (A && B) = free_var_assertion A \<union> free_var_assertion B"
+| "free_var_assertion (ImpureAnd A B) = free_var_assertion A \<union> free_var_assertion B"
+| "free_var_assertion (ImpureOr A B) = free_var_assertion A \<union> free_var_assertion B"
+| "free_var_assertion (ForAll _ A) = free_var_assertion A"
+| "free_var_assertion (Exists _ A) = free_var_assertion A"
+| "free_var_assertion (Wand A B) = free_var_assertion A \<union> free_var_assertion B"
+
+
+
 end
